update token contract

src/app/contracts/token.fst
@@ -9,39 +9,39 @@ open FStar.Mul
 module ET = Zen.ErrorT
 module Tx = Zen.TxSkeleton
 
-val cf: txSkeleton -> string -> #l:nat -> wallet l -> cost nat 15
-let cf _ _ #l _ = ret (64 + (64 + 64 + (l * 128 + 192)) + 20 + 18)
+val cf: txSkeleton -> string -> option lock -> #l:nat -> wallet l -> cost nat 15
+let cf _ _ _ #l _ = ret (64 + (64 + 64 + (l * 128 + 192)) + 19 + 22)
 
-let buy txSkeleton contractHash =
-  let pk = hashFromBase64 "DYggLLPq6eXj1YxjiPQ5dSvb/YVqAVNf8Mjnpc9P9BI=" in
+let buy txSkeleton contractHash returnAddress =
+ let! tokens = Tx.getAvailableTokens zenAsset txSkeleton in
 
-  let! tokens = Tx.getAvailableTokens zenAsset txSkeleton in
+ let txSkeleton =
+   Tx.lockToContract zenAsset tokens contractHash txSkeleton
+   >>= Tx.mint tokens contractHash
+   >>= Tx.lockToAddress contractHash tokens returnAddress in
 
-  let txSkeleton =
-    Tx.lockToContract zenAsset tokens contractHash txSkeleton
-    >>= Tx.mint tokens contractHash
-    >>= Tx.lockToPubKey contractHash tokens pk in
+ ET.retT txSkeleton
 
-  ET.retT txSkeleton
+let redeem #l txSkeleton contractHash returnAddress (wallet:wallet l) =
+ let! tokens = Tx.getAvailableTokens contractHash txSkeleton in
 
-let redeem #l txSkeleton contractHash (wallet:wallet l) =
-  let pk = hashFromBase64 "DYggLLPq6eXj1YxjiPQ5dSvb/YVqAVNf8Mjnpc9P9BI=" in
+ let txSkeleton =
+   Tx.destroy tokens contractHash txSkeleton
+   >>= Tx.lockToAddress zenAsset tokens returnAddress
+   >>= Tx.fromWallet zenAsset tokens contractHash wallet in
 
-  let! tokens = Tx.getAvailableTokens contractHash txSkeleton in
+ ET.of_optionT "contract doesn't have enough zens to pay you" txSkeleton
 
-  let txSkeleton =
-    Tx.destroy tokens contractHash txSkeleton
-    >>= Tx.lockToPubKey zenAsset tokens pk
-    >>= Tx.fromWallet zenAsset tokens contractHash wallet in
-
-  ET.of_optionT "contract doesn't have enough zens to pay you" txSkeleton
-
-val main: txSkeleton -> hash -> string -> #l:nat -> wallet l -> cost (result txSkeleton) (64 + (64 + 64 + (l * 128 + 192)) + 20 + 18)
-let main txSkeleton contractHash command #l wallet =
-  if command = "redeem" then
-    redeem txSkeleton contractHash wallet
-  else if command = "" || command = "buy" then
-    buy txSkeleton contractHash
-    |> autoInc
-  else
-    ET.autoFailw "unsupported command"
+val main: txSkeleton -> hash -> string -> option lock -> #l:nat -> wallet l -> cost (result txSkeleton) (64 + (64 + 64 + (l * 128 + 192)) + 19 + 22)
+let main txSkeleton contractHash command returnAddress #l wallet =
+ match returnAddress with
+ | Some returnAddress ->
+     if command = "redeem" then
+       redeem txSkeleton contractHash returnAddress wallet
+     else if command = "" || command = "buy" then
+       buy txSkeleton contractHash returnAddress
+       |> autoInc
+     else
+       ET.autoFailw "unsupported command"
+ | None ->
+     ET.autoFailw "returnAddress is required"
